[minor] WIP porting relational encoding to allocation machine.
Stopped transcribing in the middle of FaultRoutine.v. There's at least
two definitions that need to be adapted there. Planning to get back to
this after PL Club.

pico-ifc-coq/dyn_allocation/CLattices.v
@@ -1,7 +1,7 @@
 Require Import ZArith.
 Require Import List.
-Import ListNotations. 
-Require Import LibTactics. 
+Import ListNotations.
+Require Import LibTactics.
 
 Require Import Instr Memory.
 Require Import Lattices.
@@ -10,7 +10,7 @@ Require Import CodeGen.
 Require Import CodeSpecs.
 Require Import CodeTriples.
 
-Local Open Scope Z_scope. 
+Local Open Scope Z_scope.
 
 Section fix_cblock.
 
@@ -19,22 +19,24 @@ Variable stamp_cblock : Mem.stamp cblock = Kernel.
 
 (* Lattice-dependent parameters *)
 Class ConcreteLattice (T: Type) :=
-{ labToZ :  T -> Z
-; ZToLab :  Z -> T
+{ labToZ :  T -> Z -> memory -> Prop
+; ZToLab :  Z -> memory -> T
 ; genBot : list Instr
-; genJoin : list Instr 
+; genJoin : list Instr
 ; genFlows : list Instr
 }.
 
+Local Open Scope Z_scope.
+
 Instance TMUHL : ConcreteLattice Lab :=
 {
-  labToZ l :=
+  labToZ l z m :=
     match l with
-      | L => boolToZ false
-      | H => boolToZ true
+      | L => boolToZ false = z
+      | H => boolToZ true = z
     end
- 
-  ;ZToLab z :=
+
+  ;ZToLab z m :=
     match z with
       | 0 => L
       | _ => H
@@ -47,90 +49,153 @@ Instance TMUHL : ConcreteLattice Lab :=
   ;genFlows := genImpl
 }.
 
+Inductive mem_def_on_cache (m : memory) : Prop :=
+| mdoc_intro :
+    forall opcode pctag tag1 tag2 tag3 tagr tagrpc,
+      value_on_cache cblock m addrOpLabel (Vint opcode) ->
+      value_on_cache cblock m addrTag1 (Vint tag1) ->
+      value_on_cache cblock m addrTag2 (Vint tag2) ->
+      value_on_cache cblock m addrTag3 (Vint tag3) ->
+      value_on_cache cblock m addrTagPC (Vint pctag) ->
+      value_on_cache cblock m addrTagRes tagr ->
+      value_on_cache cblock m addrTagResPC tagrpc ->
+      mem_def_on_cache m.
+
+Lemma extends_mem_def_on_cache : forall m m',
+                                   mem_def_on_cache m ->
+                                   extends m m' ->
+                                   mem_def_on_cache m'.
+Proof.
+  intros m m' H EXT.
+  destruct H.
+  repeat match goal with
+           | H : value_on_cache _ _ _ _ |- _ => inv H
+         end.
+  econstructor; econstructor; apply EXT; eauto.
+Qed.
+
+Inductive mem_eq_except_cache (m m' : memory) : Prop :=
+| meec_intro :
+    mem_def_on_cache m ->
+    (forall b addr v,
+       b <> cblock ->
+       load b addr m = Some v ->
+       load b addr m' = Some v) ->
+    mem_eq_except_cache m m'.
+
 Class WfConcreteLattice (T: Type) (L : JoinSemiLattice T) (CL: ConcreteLattice T) :=
-{ ZToLab_labToZ_id: forall l, l = ZToLab (labToZ l)
-; genBot_spec: forall m0 s0,
+{ labToZ_cache : forall l z m m', labToZ l z m -> mem_eq_except_cache m m' -> labToZ l z m'
+; labToZ_inj : forall l1 l2 z m, labToZ l1 z m -> labToZ l2 z m -> l1 = l2
+; labToZ_ZToLab_id : forall l z m, labToZ l z m -> ZToLab z m = l
+; labToZ_extension_comp : forall m1 m2 l z,  labToZ l z m1 -> extends m1 m2 ->
+                                             mem_def_on_cache m1 ->
+                                             labToZ l z m2
+; genBot_spec: forall m0 (Hm0: mem_def_on_cache m0) (Q:memory->stack->Prop),
    HT cblock genBot
-       (fun m s => m = m0 /\ s = s0)
-       (fun m s => m = m0 /\ s = CData (Vint (labToZ bot), handlerTag) :: s0)
-; genJoin_spec: forall l l' m0 s0,
-   HT cblock genJoin
-       (fun m s => m = m0 /\
-                   s = CData (Vint (labToZ l), handlerTag) ::
-                       CData (Vint (labToZ l'), handlerTag) :: s0)
-       (fun m s => m = m0 /\
-                   s = CData (Vint (labToZ (join l l')), handlerTag) :: s0)
+      (fun m s => extends m0 m /\
+                  (forall m1 z, extends m m1 -> labToZ bot z m1 -> Q m1 ((Vint z,handlerTag):::s)))
+      Q
+; genJoin_spec:
+    forall m0 (Hm0: mem_def_on_cache m0) (Q: memory-> stack->Prop),
+       HT cblock genJoin
+         (fun m s =>
+          exists s0 l z t l' z' t',
+             s = (Vint z, t) ::: (Vint z', t') ::: s0 /\
+             extends m0 m /\
+             labToZ l z m /\ labToZ l' z' m /\
+             (forall m1 zz', extends m m1 -> labToZ (l \_/ l') zz' m1 ->
+                         Q m1 ((Vint zz', handlerTag) ::: s0)))
+         Q
+
   (* NC: we could discharge this by implementing [genFlows] in terms of
    [genJoin], and using the fact that [flows l l' = true <-> join l l' = l']. *)
-; genFlows_spec: forall l l' m0 s0,
-   HT cblock genFlows
-       (fun m s => m = m0 /\
-                   s = CData (Vint (labToZ l), handlerTag) ::
-                       CData (Vint (labToZ l'), handlerTag) :: s0)
-       (fun m s => m = m0 /\
-                   s = CData (Vint (boolToZ (flows l l')), handlerTag) :: s0)
+; genFlows_spec: forall m0 (Hm0: mem_def_on_cache m0) (Q: memory -> stack -> Prop),
+                   HT  cblock genFlows
+                       (fun m s =>
+                          exists l l' z z' t t' s0,
+                            extends m0 m /\
+                            labToZ l z m /\ labToZ l' z' m /\
+                            s = (Vint z,t):::(Vint z',t'):::s0 /\
+                            Q m ((Vint (boolToZ(flows l l')),handlerTag):::s0))
+                       Q
 }.
 
-Lemma labToZ_inj: forall {L J C} {W: WfConcreteLattice L J C} (l1 l2: L),
-  labToZ l1 = labToZ l2 -> l1 = l2.
+Section Spec_alt.
+
+Context {T: Type}
+        {Latt: JoinSemiLattice T}
+        {CLatt: ConcreteLattice T}
+        {WfCLatt: WfConcreteLattice T Latt CLatt}.
+
+Lemma genBot_spec': forall I m0 (Hm0: mem_def_on_cache m0)
+                      (Hext: extension_comp I),
+                 HT cblock genBot
+                    (fun m s => extends m0 m /\ I m s)
+                    (fun m s =>
+                       match s with
+                           | CData (Vint z,t)::tl => extends m0 m /\
+                             I m tl /\ labToZ bot z m /\ t = handlerTag
+                           | _ => False
+                       end).
 Proof.
   intros.
-  rewrite (ZToLab_labToZ_id l1).
-  rewrite (ZToLab_labToZ_id l2).
-  apply f_equal; auto.
+  eapply HT_strengthen_premise.
+  eapply genBot_spec with (m1 := m0); eauto.
+  intros. simpl.
+  destruct H.
+  intuition eauto.
+  unfold extends; eauto.
 Qed.
 
-Lemma ZToLab_labToZ_id' : forall l, l = ZToLab (labToZ l).
+Lemma genJoin_spec': forall l l' I m0 (Hmem0: mem_def_on_cache m0)
+                       (Hext: extension_comp I),
+                  HT  cblock genJoin
+                      (fun m s =>
+                         match s with
+                             | CData (Vint z,t)::CData (Vint z',t')::tl =>
+                               labToZ l z m /\ labToZ l' z' m /\
+                               extends m0 m /\ I m tl
+                             | _ => False
+                         end)
+                      (fun m s =>
+                         match s with
+                             | CData (Vint zz', t) :: tl =>
+                               labToZ (join l l') zz' m /\
+                               extends m0 m /\ I m tl
+                             | _ => False
+                         end).
 Proof.
   intros.
-  destruct l; auto.
+  eapply HT_strengthen_premise.
+  eapply genJoin_spec; eauto.
+  go_match. do 7 eexists; intuition; eauto.
+  unfold extends; eauto.
 Qed.
 
-Lemma genBot_spec' : forall m0 s0,
-   HT cblock genBot
-       (fun m s => m = m0 /\ s = s0)
-       (fun m s => m = m0 /\ s = CData (Vint (labToZ bot), handlerTag) :: s0).
-Proof.
-   intros.
-   unfold genBot, TMUHL. 
-   eapply genFalse_spec; simpl; eauto.
-Qed.
-
-Lemma genJoin_spec' : forall l l' m0 s0,
-   HT cblock genJoin
-       (fun m s => m = m0 /\
-                   s = CData (Vint (labToZ l), handlerTag) ::
-                       CData (Vint (labToZ l'), handlerTag) :: s0)
-       (fun m s => m = m0 /\
-                   s = CData (Vint (labToZ (join l l')), handlerTag) :: s0).
-Proof.
-  intros.
-  unfold genJoin, TMUHL. 
-  cases l; cases l'; unfold labToZ in *;
-    eapply HT_weaken_conclusion;
-    try (eapply genOr_spec); simpl; eauto.
-Qed.
-
-Lemma genFlows_spec': forall l l' m0 s0,
-   HT  cblock genFlows
-       (fun m s => m = m0 /\
-                   s = CData (Vint (labToZ l), handlerTag) ::
-                       CData (Vint (labToZ l'), handlerTag) :: s0)
-       (fun m s => m = m0 /\
-                   s = CData (Vint (boolToZ (flows l l')), handlerTag) :: s0).
+Lemma genFlows_spec' : forall l l' I m0 (Hmem0: mem_def_on_cache m0)
+                        (Hext: extension_comp I),
+                   HT  cblock genFlows
+                       (fun m s =>
+                          match s with
+                            | CData (Vint z,t)::CData (Vint z',t')::tl =>
+                              labToZ l z m /\ labToZ l' z' m /\
+                              extends m0 m /\ I m tl
+                            | _ => False
+                          end)
+                       (fun m s =>
+                          match s with
+                            | CData (Vint z, t) :: tl =>
+                              boolToZ (flows l l') = z /\
+                              extends m0 m /\ I m tl
+                            | _ => False
+                          end).
 Proof.
   intros.
-  unfold genFlows, TMUHL.
-  cases l; cases l'; unfold labToZ in *;
-    eapply HT_weaken_conclusion;
-    try (eapply genImpl_spec); simpl; eauto.
+  eapply HT_strengthen_premise.
+  eapply genFlows_spec; eauto.
+  go_match. do 7 eexists; intuition; eauto.
 Qed.
 
-Instance TMUHLwf : WfConcreteLattice Lab HL TMUHL :=
-{ ZToLab_labToZ_id := ZToLab_labToZ_id'
-; genBot_spec := genBot_spec'
-; genJoin_spec := genJoin_spec'
-; genFlows_spec := genFlows_spec'
-}.
+End Spec_alt.
 
 End fix_cblock.
