pico-ifc-coq/dyn_allocation/Concrete.v
@@ -28,8 +28,8 @@ Notation block := (block privilege).
 
 Variable cblock : block.
 
-Inductive CStkElmt := 
-| CData : Atom -> CStkElmt 
+Inductive CStkElmt :=
+| CData : Atom -> CStkElmt
 | CRet : PcAtom -> bool -> bool -> CStkElmt.
 (* first bool is the type of call (v/void return), second bool is
        saved privilege bit *)
@@ -51,7 +51,7 @@ Inductive CEvent :=
 (** * Cache handling mechanism *)
 
 Definition opCodeToZ (opcode : OpCode) : Z :=
-match opcode with 
+match opcode with
 | OpNoop     => 0
 | OpAdd      => 1
 | OpSub      => 2
@@ -83,21 +83,21 @@ Definition addrTagPC    := 4.
 Definition addrTagRes   := 5.
 Definition addrTagResPC := 6.
 
-(* 
+(*
 APT: non longer relevant, now that we have split memories.
 Definition tmuCacheSize := 7.
-Definition privInstSize := 1000. 
-  APT: arbitrary for now, but must be >= size of fault handler code 
-   DD: If we use this for specifying the complete execution of the fault handler, 
-   I suspect we want to give the exact size? 
+Definition privInstSize := 1000.
+  APT: arbitrary for now, but must be >= size of fault handler code
+   DD: If we use this for specifying the complete execution of the fault handler,
+   I suspect we want to give the exact size?
 *)
 
-(* APT: It should be possible for this to be a completely arbitrary integers, 
+(* APT: It should be possible for this to be a completely arbitrary integers,
 since it will never be inspected. *)
-Definition handlerTag := 42%Z. 
+Definition handlerTag := 42%Z.
 Definition dontCare := (-1)%Z.
 
-(* Build the cache line from mvector parameters. 
+(* Build the cache line from mvector parameters.
 NB: Ordering of parameters in memory must match addr* definitions above. *)
 
 Section WithListNotations.
@@ -109,50 +109,48 @@ Import ListNotations.
    in the input and output parts of the cache line come first; here,
    they come last.  This would be easy but a bit tedious to fix. *)
 
-Definition build_cache (opcode: Z) (tags: Z * Z * Z) (pctag:Z): list Atom := 
-let '(tag1,tag2,tag3) := tags in 
-[(Vint opcode,handlerTag); 
+Definition build_cache (opcode: Z) (tags: Z * Z * Z) (pctag:Z): list Atom :=
+let '(tag1,tag2,tag3) := tags in
+[(Vint opcode,handlerTag);
   (Vint tag1,handlerTag);
   (Vint tag2,handlerTag);
-  (Vint tag3,handlerTag); 
+  (Vint tag3,handlerTag);
   (Vint pctag,handlerTag);
   (Vint dontCare,handlerTag);
-  (Vint dontCare,handlerTag)]. 
+  (Vint dontCare,handlerTag)].
 
 End WithListNotations.
 
 (** Cache spec when reading from, writing to *)
-Inductive tag_in_mem (m: list Atom) addr tagv : Prop := 
-| tim_intro : index_list_Z addr m = Some (tagv,handlerTag) ->
+Inductive tag_in_mem (m: list Atom) addr tagv : Prop :=
+| tim_intro : forall t, index_list_Z addr m = Some (tagv,t) ->
               tag_in_mem m addr tagv.
 
+Inductive value_on_cache (m : memory) addr v : Prop :=
+| voc_intro : forall t, load cblock addr m = Some (v, t) ->
+                        value_on_cache m addr v.
 
-(** Cache spec when reading from, writing to *)
-Inductive tag_in_mem' (m: list Atom) addr tagv : Prop := 
-| tim_intro' : forall t, index_list_Z addr m = Some (tagv,t) ->
-               tag_in_mem' m addr tagv.
-
-(* Tests the cache line *)  
-Inductive cache_hit (m: list Atom) opcode tags pctag : Prop := 
+(* Tests the cache line *)
+Inductive cache_hit (m: list Atom) opcode tags pctag : Prop :=
 | ch_intro: forall tag1 tag2 tag3 tagr tagrpc
                      (UNPACK : tags = (tag1,tag2,tag3))
-                     (OP: tag_in_mem m addrOpLabel (Vint opcode)) 
+                     (OP: tag_in_mem m addrOpLabel (Vint opcode))
                      (TAG1: tag_in_mem m addrTag1 (Vint tag1))
                      (TAG2: tag_in_mem m addrTag2 (Vint tag2))
                      (TAG3: tag_in_mem m addrTag3 (Vint tag3))
                      (TAGPC: tag_in_mem m addrTagPC (Vint pctag))
                      (TAGR: tag_in_mem m addrTagRes (Vint tagr))
                      (TAGRPC: tag_in_mem m addrTagResPC (Vint tagrpc)),
-                cache_hit m opcode tags pctag. 
+                cache_hit m opcode tags pctag.
 
 Lemma build_cache_hit: forall opcode tags pctag,
-     cache_hit (build_cache opcode tags pctag) opcode tags pctag.                          
+     cache_hit (build_cache opcode tags pctag) opcode tags pctag.
 Proof.
-  intros. unfold build_cache. 
+  intros. unfold build_cache.
   destruct tags as [[tag1 tag2] tag3] eqn:?.
-  econstructor; eauto; 
+  econstructor; eauto;
   try unfold addrOpLabel; try unfold addrTag1; try unfold addrTag2; try unfold addrTag3;
-  try unfold addrTagPC; unfold index_list_Z; econstructor; reflexivity. 
+  try unfold addrTagPC; unfold index_list_Z; econstructor; reflexivity.
 Qed.
 
 (* Reads the cache line *)
@@ -165,10 +163,10 @@ Inductive cache_hit_read (m: list Atom) : Z -> Z -> Prop :=
 Definition update_mem_only_cache (m m': memory) :=
   forall b, b <> cblock -> Mem.get_frame m' b = Mem.get_frame m b.
 
-Definition update_cache_spec_mvec (m m': memory) := 
+Definition update_cache_spec_mvec (m m': memory) :=
   update_mem_only_cache m m' /\
   (forall addr, addr <> addrOpLabel ->
-                addr <> addrTagPC   -> 
+                addr <> addrTagPC   ->
                 addr <> addrTag1    ->
                 addr <> addrTag2    ->
                 addr <> addrTag3    ->
@@ -195,7 +193,7 @@ Definition cache_hit_read_mem (m:memory) (tagr:Z) (tagrpc:Z) : Prop :=
 (** Machine operations for popping the stack when executing a return instruction.
     And it specs. *)
 
-Inductive c_pop_to_return : list CStkElmt -> list CStkElmt -> Prop := 
+Inductive c_pop_to_return : list CStkElmt -> list CStkElmt -> Prop :=
 | cptr_done: forall a b p s,
    c_pop_to_return ((CRet a b p)::s) ((CRet a b p)::s)
 | cptr_pop: forall a s s',
@@ -207,15 +205,15 @@ Lemma c_pop_to_return_ret : forall s1 s2,
   exists a b p s, s2 = (CRet a b p)::s.
 Proof.
   induction 1; intros; simpl; eauto.
-Qed.  
-  
+Qed.
+
 Lemma c_pop_to_return_spec : forall s1 s2,
   c_pop_to_return s1 s2 ->
-  exists dstk, exists stk a b p,   
+  exists dstk, exists stk a b p,
     s1 = dstk++(CRet a b p)::stk
     /\ (forall e, In e dstk -> exists a, e = CData a).
 Proof.
-  induction 1; intros; simpl in *. 
+  induction 1; intros; simpl in *.
   exists nil ; exists s ; exists a ; exists b ; exists p.
   simpl ; split ; eauto.
   intuition.
@@ -237,7 +235,7 @@ Lemma c_pop_to_return_spec2: forall  s1 s2 p1 p2 b1 b2 a1 a2 dstk,
 Proof.
   induction dstk; intros.
   inv H. auto.
-  simpl in *. 
+  simpl in *.
   inv H. destruct (H0 (CRet a2 b2 p2)). intuition. inv H.
   eapply IHdstk; eauto.
 Qed.
@@ -249,12 +247,12 @@ Lemma c_pop_to_return_spec3: forall s1 s2 b1 b2 p1 p2 a1 a2 dstk,
 Proof.
   induction dstk; intros.
   inv H. auto.
-  simpl in *. 
+  simpl in *.
   inv H. destruct (H0 (CRet a2 b2 p2)). intuition. inv H.
   eapply IHdstk; eauto.
 Qed.
 
-Lemma c_pop_to_return_pops_data: forall cdstk a b p cs,   
+Lemma c_pop_to_return_pops_data: forall cdstk a b p cs,
      (forall a : CStkElmt, In a cdstk -> exists d : Atom, a = CData d) ->
      c_pop_to_return (cdstk ++ CRet a b p :: cs) (CRet a b p :: cs).
 Proof.
@@ -271,6 +269,6 @@ Qed.
 End CMach.
 
 Notation read_m := index_list_Z.
-Notation upd_m := update_list_Z. 
+Notation upd_m := update_list_Z.
 Notation "a ::: b" := ((CData a) :: b)  (at level 60, right associativity).
 Hint Constructors cache_hit cache_hit_read.
