pico-ifc-coq/dyn_allocation/FaultRoutine.v
@@ -12,7 +12,7 @@ Require Import ConcreteMachine.
 Require Import Rules.
 Require Import CLattices.
 Require Import CodeTriples.
-Require Import CodeSpecs. 
+Require Import CodeSpecs.
 Require Import CodeGen.
 Require Import CLattices.
 Require Import ConcreteExecutions.
@@ -22,7 +22,7 @@ Notation memory := (Mem.t Atom privilege).
 Notation PcAtom := (PcAtom Z).
 Notation block := (block privilege).
 
-Section TMU. 
+Section TMU.
 
 Open Local Scope Z_scope.
 
@@ -37,7 +37,7 @@ Notation GT := (GT cblock).
 Context {T: Type}
         {Latt: JoinSemiLattice T}
         {CLatt: ConcreteLattice T}
-        {WFCLatt: WfConcreteLattice cblock T Latt CLatt}. 
+        {WFCLatt: WfConcreteLattice cblock T Latt CLatt}.
 
 
 (* --------------------- TMU Fault Handler code ----------------------------------- *)
@@ -65,18 +65,19 @@ Fixpoint genExpr {n:nat} (e: rule_expr n) :=
   | L_Join e1 e2 => genExpr e2 ++ genExpr e1 ++ genJoin
  end.
 
-Fixpoint genCond {n:nat} (s: rule_cond n) : code :=
+Fixpoint genScond {n:nat} (s: rule_cond n) : code :=
   match s with
   | A_True => genTrue
+  | A_False => genFalse
   | A_LE e1 e2 => genExpr e2 ++ genExpr e1 ++ genFlows
-  | A_And s1 s2 => genCond s2 ++ genCond s1 ++ genAnd 
-  | A_Or s1 s2 => genCond s2 ++ genCond s1 ++ genOr 
+  | A_And s1 s2 => genScond s2 ++ genScond s1 ++ genAnd
+  | A_Or s1 s2 => genScond s2 ++ genScond s1 ++ genOr
   end.
 
 
 Definition genApplyRule {n:nat} (am:AllowModify n): code :=
-  ite (genCond (allow am))
-      (some 
+  ite (genScond (allow am))
+      (some
         (genExpr (labResPC am) ++
          genExpr (labRes am))
       )
@@ -158,10 +159,11 @@ Import Vector.VectorNotations.
 Local Open Scope nat_scope.
 
 
-Definition nth_labToZ {n:nat} (vls: Vector.t T n) (m:nat) : Z :=
-  match le_lt_dec n m with
-  | left _ => dontCare
-  | right p => labToZ (Vector.nth_order vls p)
+Definition nth_labToZ {n:nat} (vls: Vector.t T n) (s:nat) : Z -> memory -> Prop :=
+  fun z m =>
+    match le_lt_dec n s with
+      | left _ => z = dontCare
+      | right p => labToZ (Vector.nth_order vls p) z m
   end.
 
 Lemma of_nat_lt_proof_irrel:
@@ -202,187 +204,312 @@ Proof.
   erewrite nth_order_proof_irrel; eauto.
 Qed.
 
-
-Definition labsToZs {n:nat} (vls :Vector.t T n) : (Z * Z * Z) :=
-(nth_labToZ vls 0,
- nth_labToZ vls 1,
- nth_labToZ vls 2).
+Definition labsToZs {n:nat} (vls :Vector.t T n) (m: memory) : (Z * Z * Z) -> Prop :=
+fun z0z1z2 =>
+  let '(z0,z1,z2) := z0z1z2 in
+  nth_labToZ vls 0 z0 m /\
+  nth_labToZ vls 1 z1 m /\
+  nth_labToZ vls 2 z2 m.
 
 End Glue.
 
 Section TMUSpecs.
 
-Definition handlerLabel := bot. 
-
-Definition handler_initial_mem_matches 
-           (opcode: Z)
-           (tag1: Z) (tag2: Z) (tag3: Z) (pctag: Z) 
-           (m: memory) : Prop := 
-  exists cache,
-    cget m = Some cache /\
-     (exists tag, index_list_Z addrOpLabel cache = Some (Vint opcode,tag))
-  /\ (exists tag, index_list_Z addrTag1 cache = Some (Vint tag1,tag))
-  /\ (exists tag, index_list_Z addrTag2 cache = Some (Vint tag2,tag))
-  /\ (exists tag, index_list_Z addrTag3 cache = Some (Vint tag3,tag))
-  /\ (exists tag, index_list_Z addrTagPC cache = Some (Vint pctag,tag))
-.
-
-
-(* APT: Just a little sanity check that these definitions are somewhat coherent. *)
-Lemma init_init: forall (m:memory)  op ts tpc, cache_hit_mem m op ts tpc ->
-let '(l1,l2,l3) := ts in
-handler_initial_mem_matches op l1 l2 l3 tpc m.
-Proof.
-  unfold Concrete.cache_hit_mem.
-  intros.
-  destruct (Mem.get_frame m cblock) eqn:E; try (elim H; fail).  
-  inv H. inv OP. inv TAG1. inv TAG2. inv TAG3. inv TAGPC. 
-  econstructor; jauto.
-Qed.
-
+Inductive handler_initial_mem_matches
+            (opcode: Z)
+            (tag1: Z) (tag2: Z) (tag3: Z) (pctag: Z)
+            (m: memory) : Prop :=
+| hiim_intro : forall
+                 (HOPCODE : value_on_cache cblock m addrOpLabel (Vint opcode))
+                 (HTAG1 : value_on_cache cblock m addrTag1 (Vint tag1))
+                 (HTAG2 : value_on_cache cblock m addrTag2 (Vint tag2))
+                 (HTAG3 : value_on_cache cblock m addrTag3 (Vint tag3))
+                 (HPC : value_on_cache cblock m addrTagPC (Vint pctag)),
+                 handler_initial_mem_matches opcode tag1 tag2 tag3 pctag m.
+Hint Constructors handler_initial_mem_matches.
 
 (* Connecting to the definition used in ConcreteMachine.v *)
-Lemma init_enough: forall {n} (vls:Vector.t T n) m opcode pcl,
-    cache_hit_mem m (opCodeToZ opcode) (labsToZs vls) (labToZ pcl) ->
-    handler_initial_mem_matches 
-      (opCodeToZ opcode) 
-      (nth_labToZ vls 0)  
-      (nth_labToZ vls 1)
-      (nth_labToZ vls 2)
-      (labToZ pcl)
-      m.
+Lemma init_enough: forall {n} (vls:Vector.t T n) m opcode pcl z0 z1 z2 zpc,
+                   forall (Hvls: labsToZs vls m (z0,z1,z2))
+                          (Hpcl: labToZ pcl zpc m),
+    cache_hit_mem m (opCodeToZ opcode) (z0,z1,z2) zpc ->
+    handler_initial_mem_matches (opCodeToZ opcode) z0 z1 z2 zpc m.
 Proof.
-  intros. unfold labsToZs in H. 
-  unfold Concrete.cache_hit_mem in *.
-  destruct (Mem.get_frame m cblock) eqn:E; try (intuition; fail).
-  inv H. inv UNPACK. inv OP. inv TAG1. inv TAG2. inv TAG3. inv TAGPC. 
-  econstructor; jauto.
+  intros. destruct Hvls as [Hz0 [Hz1 Hz2]].
+  unfold Concrete.cache_hit_mem,
+         ConcreteMachine.cget in *.
+  destruct (Mem.get_frame m cblock) as [cache|] eqn:E; inv H.
+  inv UNPACK. inv OP. inv TAG1. inv TAG2. inv TAG3. inv TAGPC.
+  econstructor; econstructor; unfold load; rewrite E; jauto.
 Qed.
 
 Variable fetch_rule_impl: fetch_rule_impl_type.
 Variable (opcode: OpCode).
-Definition n := projT1 (fetch_rule_impl opcode).
-Definition am := projT2 (fetch_rule_impl opcode).
+Let n := projT1 (fetch_rule_impl opcode).
+Let am := projT2 (fetch_rule_impl opcode).
 Variable (vls: Vector.t T n).
 Variable (pcl: T).
+Let eval_var := mk_eval_var vls pcl.
+
+Inductive INIT_MEM (m0 : memory) : Prop :=
+| IM_intro :
+    forall z0 z1 z2 zpc zr zrpc
+           (Hz0 : nth_labToZ vls 0 z0 m0)
+           (Hz1 : nth_labToZ vls 1 z1 m0)
+           (Hz2 : nth_labToZ vls 2 z2 m0)
+           (Hpc : labToZ pcl zpc m0)
+           (Hhandler : handler_initial_mem_matches (opCodeToZ opcode)
+                                                   z0 z1 z2 zpc
+                                                   m0),
+      value_on_cache cblock m0 addrTagResPC zrpc ->
+      value_on_cache cblock m0 addrTagRes zr ->
+      INIT_MEM m0.
+Hint Constructors INIT_MEM.
+
 Variable (m0: memory).
+Hypothesis initial_m0 : INIT_MEM m0.
 
-Hypothesis initial_mem_matches:
-  handler_initial_mem_matches
-    (opCodeToZ opcode)
-    (nth_labToZ vls 0)
-    (nth_labToZ vls 1)
-    (nth_labToZ vls 2)
-    (labToZ pcl) m0.
-
-Definition eval_var := mk_eval_var vls pcl.
-
+(*
 Ltac clean_up_initial_mem :=
   unfold handler_initial_mem_matches in *;
   intuition;
   generalize initial_mem_matches; intros HH; clear initial_mem_matches;
   jauto_set_hyps; intros.
+*)
 
+Lemma extension_comp_nth_labToZ : forall m1 m2 (n m:nat) (vls: Vector.t T n) z,
+    nth_labToZ vls m z m1 ->
+    extends m1 m2 ->
+    mem_def_on_cache cblock m1 ->
+    nth_labToZ vls m z m2.
+Proof.
+  unfold nth_labToZ; intros.
+  destruct (le_lt_dec n0 m); eauto.
+  eapply labToZ_extension_comp; eauto.
+Qed.
+
+Lemma extension_comp_value_on_cache :
+  forall m1 m2 addr v,
+    value_on_cache cblock m1 addr v ->
+    extends m1 m2 ->
+    value_on_cache cblock m2 addr v.
+Proof.
+  intros m1 m2 addr v H1 H2. inv H1. econstructor. eauto.
+Qed.
+Hint Resolve extension_comp_value_on_cache.
+
+Lemma extension_comp_INIT_MEM : forall m1 m2,
+    INIT_MEM m1 ->
+    extends m1 m2 ->
+    INIT_MEM m2.
+Proof.
+  intros.
+  destruct H.
+  inv Hhandler.
+  assert (Hm1 : mem_def_on_cache cblock m1) by (econstructor; eauto).
+  econstructor; eauto 7 using extension_comp_nth_labToZ, labToZ_extension_comp.
+Qed.
+
+Lemma INIT_MEM_def_on_cache: forall m, INIT_MEM m -> mem_def_on_cache cblock m.
+Proof.
+  intros m H. destruct H. inv Hhandler.
+  econstructor; eauto using extension_comp_nth_labToZ, extension_comp_value_on_cache.
+Qed.
+
+(* genVar is only loading things on the stack, so no need
+   of the memory extension hyp of I *)
 Lemma genVar_spec:
   forall v l,
     eval_var v = l ->
-    forall s0,
-      HT  (genVar v)
-           (fun m s => m = m0 /\
-                       s = s0)
-           (fun m s => m = m0 /\
-                       s = CData (Vint (labToZ l), handlerTag) :: s0).
+    forall I,
+      HT (genVar v)
+         (fun m s => extends m0 m /\ I m s)
+         (fun m s =>
+            match s with
+              | (Vint z,t) ::: tl => extends m0 m /\
+                                labToZ l z m /\
+                                I m tl
+              | _ => False
+            end).
 Proof.
-  intros v l Heval_var s0.
-
-  clean_up_initial_mem.
-
-  destruct v; simpl; eapply loadFromCache_spec;
-  simpl in *; unfold load; auto;
-  unfold ConcreteMachine.cget in *; rewrite H.
-
-  (* Most of the cases are very similar ... *)
-  Ltac nth_order_case k :=
-    erewrite (nth_order_valid n vls k) in *;
-    intuition;
-    subst; auto;
-    eauto.
-
-  nth_order_case 0%nat.
-  nth_order_case 1%nat.
-  nth_order_case 2%nat.
-
-  subst; eauto.
+  intros v l Heval_var I.
+  destruct initial_m0.
+  inv Hhandler.
+  assert (Hmem0: mem_def_on_cache cblock m0) by (econstructor; eauto).
+  case_eq v; intros; subst; simpl;
+  match goal with
+    | [HH : value_on_cache cblock _ ?addr ?zz |-
+       HT (loadFromCache ?addr) _ _] =>
+       eapply HT_strengthen_premise
+              with (P:= (fun m1 s0 => value_on_cache cblock m1 addr zz /\
+                                      ((fun m s => extends m0 m /\ I m s) m1 s0)));
+       try solve [intuition eauto];
+       eapply HT_weaken_conclusion
+  end;
+  try (eapply loadFromCache_spec_I with (I := (fun m s => extends m0 m /\ I m s))); eauto;
+  simpl; intros;
+  destruct s; intuition;
+  (destruct c; intuition);
+  (destruct a; intuition);
+  subst; intuition eauto using labToZ_extension_comp;
+  unfold nth_labToZ in *;
+  repeat match goal with
+           | H : context [le_lt_dec ?n ?m] |- _ =>
+             destruct (le_lt_dec n m); try omega
+         end;
+  erewrite nth_order_proof_irrel; eauto using labToZ_extension_comp.
 Qed.
+
+Hint Resolve  extension_comp_INIT_MEM INIT_MEM_def_on_cache.
 
 Lemma genExpr_spec: forall (e: rule_expr n),
   forall l,
     eval_expr eval_var e = l ->
-    forall s0,
-      HT  (genExpr e)
-           (fun m s => m = m0 /\
-                       s = s0)
-           (fun m s => m = m0 /\
-                       s = CData (Vint (labToZ l), handlerTag) :: s0).
+    forall I
+           (Hext: extension_comp I),
+      HT   (genExpr e)
+           (fun m s => extends m0 m /\ I m s)
+           (fun m s => match s with
+                         | (Vint z, t) ::: tl => I m tl /\ labToZ l z m  /\
+                                                 extends m0 m /\ INIT_MEM m
+                         | _ => False
+                       end).
 Proof.
-  induction e; intros ? Heval_expr ?;
-    simpl; simpl in Heval_expr.
-  subst l. 
-  eapply genBot_spec; eauto. 
-  eapply genVar_spec; eauto.
-  eapply HT_compose.
-  eapply IHe2; eauto.
-  eapply HT_compose.
-  eapply IHe1; eauto.
-  rewrite <- Heval_expr.
-  eapply genJoin_spec.
-  auto.
+  induction e; intros ? Heval_expr ? Hext;
+  simpl; simpl in Heval_expr.
+  subst l.
+  - eapply HT_weaken_conclusion.
+    eapply genBot_spec' ; eauto.
+    unfold extension_comp, extends in *; intuition ; eauto.
+    go_match.
+
+  - eapply HT_weaken_conclusion.
+    eapply genVar_spec; eauto.
+    go_match.
+
+  - eapply HT_compose.
+    eapply IHe2; eauto.
+
+    eapply HT_compose.
+    + eapply HT_strengthen_premise.
+      eapply (IHe1 (eval_expr eval_var e1) (eq_refl _)
+                   (fun m s =>
+                      match s with
+                        | (Vint z,t):::tl => I m tl
+                                             /\ labToZ (eval_expr eval_var e2) z m
+                                             /\ extends m0 m /\ INIT_MEM m
+                        | _ => False
+                      end)); eauto.
+      unfold extension_comp, extends.
+      destruct s; intuition.
+      destruct c; intuition.
+      destruct a.
+      destruct v; intuition eauto using labToZ_extension_comp.
+      go_match.
+    + eapply HT_strengthen_premise.
+      eapply HT_weaken_conclusion.
+      eapply genJoin_spec'; eauto.
+      go_match.
+      go_match.
 Qed.
 
-
-Lemma genCond_spec: forall (c: rule_cond n),
+Lemma genScond_spec: forall (c: rule_cond n),
   forall b,
     eval_cond eval_var c = b ->
-    forall s0,
-      HT (genCond c)
-           (fun m s => m = m0 /\
-                       s = s0)
-           (fun m s => m = m0 /\
-                       s = CData (Vint (boolToZ b), handlerTag) :: s0).
+    forall I (Hext: extension_comp I),
+      HT   (genScond c)
+           (fun m s => extends m0 m /\ I m s)
+           (fun m s => match s with
+                           | (Vint z,t):::tl => I m tl /\ boolToZ b = z /\
+                                                extends m0 m /\ INIT_MEM m
+                           | _ => False
+                       end).
 Proof.
   induction c; intros; simpl;
     try (simpl in H); subst.
 
   (* True *)
-  eapply push_spec''.
+  eapply HT_weaken_conclusion.
+  eapply push_spec_I. go_match.
+
+  (* False *)
+  eapply HT_weaken_conclusion.
+  eapply push_spec_I. go_match.
 
   (* Flows *)
   eapply HT_compose.
-  eapply genExpr_spec.
-  eauto.
+  eapply genExpr_spec; eauto.
+
   eapply HT_compose.
-  eapply genExpr_spec.
-  eauto.
-  eapply genFlows_spec.
-  auto.
+  eapply HT_strengthen_premise; eauto.
+  eapply (genExpr_spec r (eval_expr eval_var r) (eq_refl _))
+  with
+  (I:= fun m s =>
+         match s with
+           | (Vint z, t) ::: tl => I m tl /\ labToZ (eval_expr eval_var r0) z m /\
+                                   extends m0 m
+           | _ => False
+     end).
+    unfold extension_comp, extends; simpl.
+    intros.
+    destruct s; intuition.
+    destruct c; intuition.
+    destruct a.
+    destruct v; intuition eauto using labToZ_extension_comp.
+    go_match.
+  eapply HT_consequence.
+  eapply (genFlows_spec' cblock (eval_expr eval_var r) (eval_expr eval_var r0)
+         (fun m s => extends m0 m /\ I m s)) ; eauto.
+  unfold extension_comp, extends; simpl. intuition; eauto.
+  go_match.
+  go_match.
 
   (* And *)
   eapply HT_compose.
-  eapply IHc2.
-  eauto.
-  eapply HT_compose.
-  eapply IHc1.
-  eauto.
-  eapply genAnd_spec; auto.
+  eapply IHc2; eauto.
 
-  (* Or *)
   eapply HT_compose.
-  eapply IHc2.
-  eauto.
+  eapply HT_strengthen_premise.
+  eapply (IHc1 (eval_cond eval_var c1) (eq_refl _)
+                 (fun m s =>
+                    match s with
+                      | (Vint z,t):::tl => I m tl
+                        /\ boolToZ (eval_cond eval_var c2) = z
+                        /\ extends m0 m
+                      | _ => False
+                    end)); eauto.
+  unfold extension_comp, extends; simpl.
+  intuition; eauto. go_match.
+
+  go_match.
+
+  eapply HT_consequence.
+  eapply (genAnd_spec_I) with (I:= fun m s => extends m0 m /\ I m s) ; eauto.
+  go_match.
+  go_match.
+
+    (* OR *)
   eapply HT_compose.
-  eapply IHc1.
-  eauto.
-  eapply genOr_spec; auto.
+  eapply IHc2; eauto.
+
+  eapply HT_compose.
+  eapply HT_strengthen_premise.
+  eapply (IHc1 (eval_cond eval_var c1) (eq_refl _)
+                 (fun m s =>
+                    match s with
+                      | (Vint z,t):::tl => I m tl
+                        /\ boolToZ (eval_cond eval_var c2) = z
+                        /\ extends m0 m
+                      | _ => False
+                    end)); eauto.
+  unfold extension_comp, extends; simpl.
+  intuition; eauto. go_match.
+  go_match.
+
+  eapply HT_consequence.
+  eapply (genOr_spec_I) with (I:= fun m s => extends m0 m /\ I m s) ; eauto.
+  go_match.
+  go_match.
 Qed.
 
 (* XXX: how to best model [option]s and monadic sequencing in the code
@@ -408,141 +535,217 @@ Qed.
 *)
 
 Lemma genApplyRule_spec_Some:
-  forall lrpc lr,
-    apply_rule am pcl vls = Some (lrpc, lr) ->
-    forall s0,
+  forall l1 l2,
+    apply_rule am pcl vls = Some (l1, l2) ->
+    forall I (Hext: extension_comp I),
       HT   (genApplyRule am)
-           (fun m s => m = m0 /\
-                       s = s0)
-           (fun m s => m = m0 /\
-                       s = CData (   Vint 1, handlerTag) :: (* [Some (...)] *)
-                           CData (Vint (labToZ lr), handlerTag) ::
-                           CData (Vint (labToZ lrpc), handlerTag) :: s0).
+           (fun m s => extends m0 m /\ I m s)
+           (fun m s => match s with
+                           | (Vint some1, t1) ::: (Vint zr, t3) ::: (Vint zrpc, t4) ::: tl =>
+                             1 = some1 (* [Some (...)] *)
+                             /\ labToZ l1 zrpc m /\ labToZ l2 zr m
+                             /\ extends m0 m /\ I m tl
+                           | _ => False
+                       end).
 Proof.
-  introv Happly. intros.
+  introv Happly.
   unfold genApplyRule.
   unfold apply_rule in Happly.
   cases_if in Happly.
-  inversion Happly; subst.
+  inv  Happly. intros I Hext.
 
-  eapply ite_spec_specialized with (v:=boolToZ true); auto.
-    eapply genCond_spec; auto.
+  - eapply (ite_spec_specialized_I' cblock (boolToZ true)); eauto.
 
-    intros.
+    + eapply HT_weaken_conclusion.
+      eapply (genScond_spec (allow am) true H I); eauto.
+      go_match.
 
-    eapply some_spec.
-    eapply HT_compose.
-      apply genExpr_spec.
-      eauto.
+    + intros.
+      eapply HT_weaken_conclusion.
+      eapply some_spec_I.
 
-      eapply genExpr_spec.
-      eauto.
+      eapply HT_compose.
+      eapply genExpr_spec with (I:= I); eauto.
 
-    intros; false; omega.
+      eapply HT_strengthen_premise.
+      eapply genExpr_spec with
+      (I:= fun m s => match s with
+                        | (Vint z, t) ::: tl0 =>
+                          I m tl0
+                          /\ labToZ (eval_expr eval_var (labResPC am)) z m
+                          /\ extends m0 m
+                        | _ => False
+                      end); eauto.
+      unfold extension_comp, extends in *.
+      simpl. intuition. go_match. eauto using labToZ_extension_comp.
+      go_match.
+      go_match.
+    + intros; false; omega.
 Qed.
 
 Lemma genApplyRule_spec_None:
-    apply_rule am pcl vls = None ->
-    forall s0,
+    apply_rule am pcl vls  = None ->
+    forall I (Hext: extension_comp I),
       HT   (genApplyRule am)
-           (fun m s => m = m0 /\
-                       s = s0)
-           (fun m s => m = m0 /\
-                       s = CData (Vint 0, handlerTag) :: s0). (* [None] *)
+           (fun m s => extends m0 m /\ I m s)
+           (fun m s => match s with
+                         | (Vint none1, t1) :::  tl =>
+                           0 = none1  (* [None] *)
+                           /\ extends m0 m /\ I m tl
+                         | _ => False
+                       end).
 Proof.
-  introv Happly. intros.
+  introv Happly Hext.
   unfold genApplyRule.
   unfold apply_rule in Happly.
   cases_if in Happly.
 
-  eapply ite_spec_specialized with (v:=boolToZ false); auto; intros.
-    eapply genCond_spec; auto.
+  eapply ite_spec_specialized_I' with (v:=boolToZ false); eauto; intros.
+  eapply HT_weaken_conclusion.
+  eapply genScond_spec; auto. unfold eval_var, n.
+  rewrite H.
+  go_match.
+  unfold boolToZ in *; false; try omega.
 
-    unfold boolToZ in *; false; omega.
-
-    apply none_spec.
+  eapply HT_weaken_conclusion.
+  eapply (push_spec_I cblock 0); eauto.
+  go_match.
 Qed.
 
-Definition listify_apply_rule
-  (ar: option (T * T)) (s0: stack): stack
-:=
+Definition listify_apply_rule (ar: option (T * T))
+                              (s0: stack) (zr zpc: Z) : stack -> Prop :=
   match ar with
-  | None            => CData (Vint 0, handlerTag) :: s0
-  | Some (lrpc, lr) => CData (Vint 1, handlerTag) ::
-                        CData (Vint (labToZ lr), handlerTag) ::
-                        CData (Vint (labToZ lrpc), handlerTag) :: s0
+  | None           => fun s => exists t, s = CData (Vint 0, t) :: s0
+  | Some (lpc, lr) => fun s => exists t1 t2 t3, s = CData (Vint 1, t1)   ::
+                                                    CData (Vint zr, t2)  ::
+                                                    CData (Vint zpc, t3) :: s0
+  end.
+
+Definition labToZ_rule_res (ar: option (T * T)) (zr zpc: Z) m : Prop :=
+  match ar with
+  | None           => True
+  | Some (lpc, lr) => labToZ lr zr m /\ labToZ lpc zpc m
   end.
 
 Lemma genApplyRule_spec:
   forall ar,
     apply_rule am pcl vls = ar ->
-    forall s0,
+    forall I (Hext: extension_comp I),
       HT   (genApplyRule am)
-           (fun m s => m = m0 /\
-                       s = s0)
-           (fun m s => m = m0 /\
-                       s = listify_apply_rule ar s0).
+           (fun m s => extends m0 m /\ I m s)
+           (fun m s => extends m0 m /\
+                       exists s0 zr zrpc,
+                       labToZ_rule_res ar zr zrpc m /\
+                       listify_apply_rule ar s0 zr zrpc s /\
+                       I m s0).
 Proof.
   intros.
-  case_eq ar; intros p ?; subst.
-  - destruct p as [lrpc lr].
-    eapply genApplyRule_spec_Some; eauto.
-  - eapply genApplyRule_spec_None; eauto.
+  unfold listify_apply_rule, labToZ_rule_res.
+  case_eq ar ; [intros [r rpc] | intros rpc] ; intros ; subst.
+  - eapply HT_weaken_conclusion.
+    eapply (genApplyRule_spec_Some r rpc H0 I); eauto.
+    go_match.
+    do 5 eexists; eauto.
+  - eapply HT_weaken_conclusion.
+    eapply genApplyRule_spec_None; eauto.
+    go_match. eexists. eexists 0. eexists 0.
+    eauto.
 Qed.
 
-Lemma genApplyRule_spec_GT:
+Lemma genApplyRule_spec_GT_ext:
   forall ar,
     apply_rule am pcl vls = ar ->
-      GT (genApplyRule am)
-         (fun m s => m = m0)
-         (fun m0' s0 m s => m = m0 /\
-                            s = listify_apply_rule ar s0).
+    forall (I:HProp) (Hext: extension_comp I),
+      GT_ext cblock (genApplyRule am)
+         (fun m s => extends m0 m /\ I m s)
+         (fun m0' s0 m s => extends m0 m0' /\ extends m0' m /\
+                            exists zr zrpc,
+                              labToZ_rule_res ar zr zrpc m /\
+                              listify_apply_rule ar s0 zr zrpc s /\
+                              I m s0).
 Proof.
-  unfold CodeSpecs.GT; intros.
-  eapply HT_consequence; eauto.
-  - eapply genApplyRule_spec; eauto.
-  - simpl; intuition (subst; eauto).
-  - simpl; intuition (subst; eauto).
+  unfold GT_ext; intros.
+  eapply HT_consequence.
+  eapply  (genApplyRule_spec ar H (fun m s => extends m0 m1 /\
+                                              extends m1 m /\
+                                              s = s0 /\ I m s)); eauto.
+  unfold extension_comp; eauto.
+  unfold extends in *; intuition ; eauto.
+  go_match. intuition; substs; eauto.
+  unfold extends. auto.
+  simpl. intros m s [Hm [s1 [zr [zrpc [Har Hlist]]]]].
+  intuition. substs; eauto.
 Qed.
 
-Lemma genCheckOp_spec:
-  forall opcode', forall s0,
+Lemma genCheckOp_spec_HT_ext:
+  forall opcode' I (Hext: extension_comp I),
     HT (genCheckOp opcode')
-      (fun m s => m = m0 /\
-                  s = s0)
-      (fun m s => m = m0 /\
-                  s = (Vint (boolToZ (opCodeToZ opcode' =? opCodeToZ opcode))
-                      ,handlerTag) ::: s0).
+       (fun m s => extends m0 m /\ I m s)
+       (fun m s => match s with
+                       | (Vint z,t):::tl =>
+                         extends m0 m /\
+                         boolToZ (opCodeToZ opcode' =? opCodeToZ opcode) = z /\
+                         I m tl
+                       | _ => False
+                   end).
 Proof.
-  clean_up_initial_mem.
-  intros.
+  destruct initial_m0.
+  inv Hhandler. intuition.
   unfold genCheckOp.
-  eapply genTestEqual_spec; auto.
-  eapply push_spec''.
-  intros.
-  eapply loadFromCache_spec; auto.
-  unfold load; unfold ConcreteMachine.cget in *; rewrite H.
+  eapply genTestEqual_spec_I; try assumption. intros I' HextI'.
+  eapply HT_strengthen_premise.
+  eapply HT_weaken_conclusion.
+  eapply (push_spec_I) with (I:= fun m s => extends m0 m /\ I' m s).
+  go_match.
+  go_match. intuition.
+  intros I' HextI'.
+  eapply HT_strengthen_premise.
+  eapply HT_weaken_conclusion.
+  eapply loadFromCache_spec_I with (v := Vint (opCodeToZ opcode)) (I:= fun m s => extends m0 m /\ I' m s); eauto.
   eauto.
+  go_match.
+  go_match; intuition eauto using extension_comp_value_on_cache.
 Qed.
 
-Lemma genCheckOp_spec_GT:
-  forall opcode',
-    GT (genCheckOp opcode')
-       (fun m s => m = m0)
-       (fun m0' s0 m s => m = m0 /\
+Lemma genCheckOp_spec_GT_ext:
+  forall opcode' I (Hext: extension_comp I),
+    GT_ext cblock (genCheckOp opcode')
+       (fun m s => extends m0 m /\ I m s)
+       (fun m0' s0 m s => exists t, extends m0 m0' /\ extends m0' m /\
                           s = (Vint (boolToZ (opCodeToZ opcode' =? opCodeToZ opcode))
-                               ,handlerTag) ::: s0).
+                               ,t) ::: s0
+                          /\ I m s0).
 Proof.
-  unfold CodeSpecs.GT; intros.
-  eapply HT_consequence; eauto.
-  - eapply genCheckOp_spec; eauto.
-  - simpl; intuition (subst; eauto).
-  - simpl; intuition (subst; eauto).
+  unfold GT_ext; intros.
+  eapply HT_weaken_conclusion.
+  eapply HT_strengthen_premise.
+  eapply genCheckOp_spec_HT_ext with (I:= fun m s => extends m0 m1 /\
+                                                 extends m1 m /\
+                                                 I m s /\ s = s0).
+  unfold extension_comp, extends ; simpl ; eauto.
+  simpl; intuition (subst; eauto).
+  simpl. intuition; substs; auto.
+  unfold extends in * ; eauto.
+  unfold extends in * ; eauto.
+  simpl. go_match.
 Qed.
+
+End TMUSpecs.
 
 Section FaultHandlerSpec.
 
 Variable ar: option (T * T).
+
+Variable fetch_rule_impl: fetch_rule_impl_type.
+Variable (opcode: OpCode).
+Let n := projT1 (fetch_rule_impl opcode).
+Let am := projT2 (fetch_rule_impl opcode).
+
+Variable (vls: Vector.t T n).
+Variable (pcl: T).
+
+Let eval_var := mk_eval_var vls pcl.
+
 Hypothesis H_apply_rule: apply_rule am pcl vls = ar.
 
 (* Don't really need to specify [Qnil] since it will never run *)
@@ -551,20 +754,29 @@ Definition genV: OpCode -> HFun :=
   fun i _ _ => boolToZ (opCodeToZ i =? opCodeToZ opcode).
 Definition genC: OpCode -> code := genCheckOp.
 Definition genB: OpCode -> code := genApplyRule' fetch_rule_impl.
-Definition genQ: OpCode -> GProp :=
-         (fun i m0' s0 m s => m = m0 /\
-                              s = listify_apply_rule ar s0).
+Definition genQ: HProp -> OpCode -> GProp :=
+         (fun I i m0' s0 m s => extends m0' m /\
+                                exists zr zrpc,
+                                  labToZ_rule_res ar zr zrpc m /\
+                                  listify_apply_rule ar s0 zr zrpc s /\ I m s0).
 
-Lemma genCheckOp_spec_GT_push_v:
-  forall opcode',
-    GT_push_v cblock (genC opcode')
-              (fun m s => m = m0)
-              (genV opcode').
+Let INIT_MEM := INIT_MEM fetch_rule_impl opcode vls pcl.
+
+Variable m0 : memory.
+Hypothesis INIT_MEM0: INIT_MEM m0.
+
+Lemma genCheckOp_spec_GT_push_v_ext:
+  forall opcode' I (Hext: extension_comp I),
+    GT_push_v_ext cblock (genC opcode')
+                  (fun m s => extends m0 m /\ I m s)
+                  (genV opcode').
 Proof.
-  intros; eapply GT_consequence'; auto.
-  eapply genCheckOp_spec_GT.
-  eauto.
-  intuition (subst; intuition).
+  intros; eapply GT_consequence'_ext; eauto.
+  eapply genCheckOp_spec_GT_ext with (I:= fun m s => extends m0 m /\ I m s); eauto.
+  unfold extension_comp, extends in *; intuition ; eauto.
+  intuition.
+  simpl.
+  split_vc.
 Qed.
 
 Lemma dec_eq_OpCode: forall (o o': OpCode),
@@ -572,7 +784,6 @@ Lemma dec_eq_OpCode: forall (o o': OpCode),
 Proof.
   destruct o; destruct o'; solve [ left; reflexivity | right; congruence ].
 Qed.
-
 
 Lemma opCodeToZ_inj: forall opcode opcode',
   (boolToZ (opCodeToZ opcode' =? opCodeToZ opcode) <> 0) ->
@@ -582,59 +793,86 @@ Proof.
   destruct o; destruct o'; simpl; solve [ auto | intros; false; omega ].
 Qed.
 
-Lemma genApplyRule'_spec_GT_guard_v:
-  forall opcode',
-    GT_guard_v cblock
-               (genB opcode')
-               (fun m s => m = m0)
+Lemma genApplyRule'_spec_GT_guard_v_ext:
+  forall opcode' I (Hext: extension_comp I),
+    GT_guard_v_ext cblock (genB opcode')
+               (fun m s => extends m0 m /\ I m s)
                (genV opcode')
-               (genQ opcode').
+               (genQ I opcode').
 Proof.
-  (* NC: This proof is ugly ... not sure where I've gone wrong, but I
-  have ... *)
   intros.
-  cases (dec_eq_OpCode opcode' opcode) as Eq; clear Eq.
-  - eapply GT_consequence'; auto.
-    + unfold genB, genApplyRule'.
-      subst opcode'.
-      fold am.
-      eapply genApplyRule_spec_GT; eauto.
-    + iauto.
-    + (* why does iauto no longer work here?? *)
-      subst ar. intros.  subst m1. econstructor. intuition. subst ar. intuition.
-  - unfold GT_guard_v, CodeSpecs.GT, CodeTriples.HT.
+  cases (dec_eq_OpCode opcode' opcode) as Eq; clear Eq. substs.
+  - eapply GT_consequence'_ext; try assumption.
+    unfold genB, genApplyRule'.
+    eapply genApplyRule_spec_GT_ext; eauto.
+    intuition.
+    simpl. intuition.
+    econstructor; eauto.
+
+  - unfold GT_guard_v_ext, GT_ext, CodeTriples.HT.
     intros.
     unfold genV in *.
     pose (opCodeToZ_inj opcode opcode').
-    false; intuition. 
-Qed. 
-
-Lemma H_indexed_hyps: indexed_hyps cblock _ genC genB genQ genV (fun m s => m = m0) opcodes.
-Proof.
-  simpl.
-  intuition; try (solve
-    [ eapply genCheckOp_spec_GT_push_v
-    | eapply genApplyRule'_spec_GT_guard_v ]).
+    false; intuition.
 Qed.
 
-Lemma genComputeResults_spec_GT:
-  GT (genComputeResults fetch_rule_impl)
-     (fun m s => m = m0)
-     (fun m0' s0 m s => m = m0 /\
-                        s = listify_apply_rule ar s0).
+
+Lemma H_indexed_hyps: forall (I:HProp) (Hext: extension_comp I),
+                        indexed_hyps_ext cblock _ genC genB (genQ I)
+                        genV (fun m s => extends m0 m /\ I m s) opcodes.
+Proof.
+  unfold indexed_hyps_ext; simpl;
+  intuition ; try (solve
+    [ (eapply GT_consequence'_ext; eauto);
+    try solve [(eapply genCheckOp_spec_GT_push_v_ext; eauto)];
+    try (simpl ; intuition ; subst ; iauto)
+    | eapply genApplyRule'_spec_GT_guard_v_ext; eauto ]).
+Qed.
+
+End FaultHandlerSpec.
+
+Variable ar: option (T * T).
+
+Variable fetch_rule_impl: fetch_rule_impl_type.
+Variable (opcode: OpCode).
+Let n := projT1 (fetch_rule_impl opcode).
+Let am := projT2 (fetch_rule_impl opcode).
+
+Variable (vls: Vector.t T n).
+Variable (pcl: T).
+
+Let eval_var := mk_eval_var vls pcl.
+
+Hypothesis H_apply_rule: apply_rule am pcl vls = ar.
+Let INIT_MEM := INIT_MEM fetch_rule_impl opcode vls pcl.
+
+Lemma genComputeResults_spec_GT_ext: forall I (Hext: extension_comp I)
+                                       m0 (INIT_MEM0: INIT_MEM m0),
+    GT_ext cblock (genComputeResults fetch_rule_impl)
+       (fun m s => extends m0 m /\ I m s)
+       (fun m0' s0 m s => extends m0 m0' /\ extends m0' m /\
+                          exists zr zpc,
+                            labToZ_rule_res ar zr zpc m /\
+                            listify_apply_rule ar s0 zr zpc s /\ I m s0).
 Proof.
   intros.
-  eapply GT_consequence'; auto.
   unfold genComputeResults.
-  eapply indexed_cases_spec with (Qnil:=Qnil); auto.
+  eapply GT_consequence'_ext; try assumption.
+  eapply indexed_cases_spec_ext with
+  (Qnil:= Qnil)
+  (genV:= genV opcode)
+  (P:= fun m s => extends m0 m /\ I m s)
+  (genQ:= genQ ar I); try assumption.
   - Case "default case that we never reach".
-    unfold CodeSpecs.GT; intros.
+    unfold GT_ext; intros.
     eapply HT_consequence.
-    eapply nop_spec.
-    iauto.
+    eapply nop_spec_I with (I:= fun m s => extends m1 m /\ I m s /\ I m1 s); eauto.
+    intros. intuition; subst.
+    unfold extends in * ; eauto.
+    eauto.
     unfold Qnil; iauto.
-  - exact H_indexed_hyps.
-  - iauto.
+  - eapply (H_indexed_hyps ar fetch_rule_impl opcode vls pcl H_apply_rule m0 INIT_MEM0  I); auto.
+  - simpl. iauto.
   - Case "untangle post condition".
     simpl.
     assert (0 = 0) by reflexivity.
@@ -644,76 +882,97 @@ Proof.
     term and says it's ill typed *)
     clear H_apply_rule.
     unfold genV, genQ.
-    destruct opcode; simpl; intuition.
+    cases opcode; simpl; intuition.
 Qed.
 
-(* Under our assumptions, [genComputeResults] just runs the appropriate
-   [genApplyRule]: *)
-Lemma genComputeResults_spec:
-    forall s0,
+Lemma genComputeResults_spec: forall I s0 m0 (INIT_MEM0: INIT_MEM m0),
+    forall (Hext: extension_comp I),
       HT   (genComputeResults fetch_rule_impl)
-           (fun m s => m = m0 /\
-                       s = s0)
-           (fun m s => m = m0 /\
-                       s = listify_apply_rule ar s0).
+           (fun m s => extends m0 m /\ s = s0 /\ I m0 s /\ I m s)
+           (fun m s => extends m0 m /\
+                       exists zr zpc,
+                         labToZ_rule_res ar zr zpc m /\
+                         listify_apply_rule ar s0 zr zpc s /\ I m s0).
 Proof.
   intros.
-  eapply HT_consequence'.
-  eapply genComputeResults_spec_GT.
-  iauto.
-  simpl; iauto.
+  eapply HT_consequence.
+  eapply (genComputeResults_spec_GT_ext I Hext m0); eauto.
+  simpl.
+
+  intros; intuition; substs; auto.
+  unfold extends; eauto. auto.
+  unfold extends; eauto.
+  intros; intuition; intuition.
 Qed.
 
-
-Lemma genStoreResults_spec_Some: forall lr lrpc,
-  valid_address cblock addrTagRes m0 ->
-  valid_address cblock addrTagResPC m0 ->
-  ar = Some (lrpc, lr) ->
-  forall s0,
-    HT genStoreResults
-       (fun m s => m = m0 /\
-                   s = listify_apply_rule ar s0)
-       (fun m s =>
-        (exists m', store cblock addrTagRes (Vint (labToZ lr),handlerTag) m0
-                    = Some m'
-                 /\ store cblock addrTagResPC (Vint (labToZ lrpc),handlerTag) m'
-                    = Some m)
-        /\ s = (Vint 1,handlerTag) ::: s0).
+(* trying in WP wtyle *)
+Lemma storeAt_spec_wp': forall a Q,
+  HT (storeAt a)
+     (fun m0 s0 => exists vl s m, s0 = vl ::: s /\
+                               store cblock a vl m0 = Some m /\
+                               Q m s)
+     Q.
 Proof.
-  introv HvalidRes HvalidResPC Har_eq; intros.
+  intros.
+  eapply HT_compose_flip.
+  eapply store_spec_wp'; eauto.
+  unfold push.
+  eapply HT_strengthen_premise.
+  eapply push_cptr_spec_wp.
+
+  intuition; eauto. destruct H as [vl [s0 [m0 Hint]]]. intuition; substs.
+  do 5 eexists; intuition; eauto.
+Qed.
+
+Lemma genStoreResults_spec_Some: forall Q,
+  forall lr lpc,
+    ar = Some (lpc,lr) ->
+      HT genStoreResults
+         (fun m s => exists s0 zr zpc,
+            labToZ_rule_res ar zr zpc m /\
+            listify_apply_rule ar s0 zr zpc s /\
+            valid_address cblock addrTagRes m /\
+            valid_address cblock addrTagResPC m /\
+            forall t1 t2,
+            exists m' m'',
+              (store cblock addrTagRes (Vint zr,t1) m = Some m')
+               /\ store cblock addrTagResPC (Vint zpc,t2) m' = Some m''
+               /\ labToZ_rule_res ar zr zpc m''
+               /\ Q m'' ((Vint 1,handlerTag):::s0))
+         Q
+.
+Proof.
+  introv Har_eq; intros.
   unfold listify_apply_rule.
   rewrite Har_eq.
   unfold genStoreResults.
-
-  (* Need to exploit early so that existentials can be unified against
-  vars introduced here *)
-  eapply valid_store in HvalidRes.
-  destruct HvalidRes as [m' ?].
-  eapply valid_address_upd in HvalidResPC.
-  eapply valid_store in HvalidResPC.
-  destruct HvalidResPC as [m'' ?]; eauto.
-
   eapply HT_strengthen_premise.
-  eapply ifNZ_spec_NZ with (v:=1).
-  eapply HT_compose_bwd.
-  eapply HT_compose_bwd.
-  eapply genTrue_spec_wp.
-  eapply storeAt_spec_wp; auto.
-  eapply storeAt_spec_wp; auto.
+  eapply ifNZ_spec_existential.
+  eapply HT_compose_flip.
+  eapply HT_compose_flip.
+  eapply genTrue_spec_wp; eauto.
+  eapply storeAt_spec_wp'.
+  eapply storeAt_spec_wp'.
+  eapply genFalse_spec_wp.
 
-  omega.
-  simpl; intuition; subst; jauto.
-  eauto.
+  intros. destruct H as [s0 [zr [zpc Hint]]]. intuition.
+  split_vc.
+  edestruct H4 as [m' [m'' Hint]]. intuition.
+  subst.
+
+  split_vc.
+  inv H7.
 Qed.
 
-Lemma genStoreResults_spec_None:
+Lemma genStoreResults_spec_None: forall Q: memory -> stack -> Prop,
   ar = None ->
-  forall s0,
     HT genStoreResults
-       (fun m s => m = m0 /\
-                   s = listify_apply_rule ar s0)
-       (fun m s => m = m0 /\
-                   s = (Vint 0,handlerTag) ::: s0).
+       (fun m s => exists s0 zr zpc,
+                     labToZ_rule_res ar zr zpc m /\
+                     listify_apply_rule ar s0 zr zpc s /\
+                     (forall m0,
+                       extends m m0 -> Q m0 ((Vint 0,handlerTag) ::: s0)))
+       Q.
 Proof.
   introv Har_eq; intros.
   unfold listify_apply_rule.
@@ -721,13 +980,22 @@ Proof.
   unfold genStoreResults.
 
   eapply HT_strengthen_premise.
-  eapply ifNZ_spec_Z with (v:=0).
-  eapply genFalse_spec.
+  eapply ifNZ_spec_existential.
 
-  reflexivity.
-  jauto.
+
+  eapply HT_compose_flip.
+  eapply HT_compose_flip.
+  eapply genTrue_spec_wp; eauto.
+  eapply storeAt_spec_wp'.
+  eapply storeAt_spec_wp'.
+  eapply genFalse_spec_wp.
+
+  intros. destruct H as [s0 [zr [zpc [t Hint]]]].
+  split_vc.
+  eauto using extends_refl.
 Qed.
 
+(* DELETE?
 (* The irrelevant memory never changes *)
 Lemma genStoreResults_update_cache_spec_rvec:
   valid_address cblock addrTagRes m0 ->
@@ -771,12 +1039,18 @@ Proof.
     simpl; intuition; subst; auto.
     intros addr NEQ. trivial.
 Qed.
+*)
 
-Definition handler_final_mem_matches (lrpc: T) (lr: T) (m: memory) (m': memory) :Prop :=
-     cache_hit_read_mem cblock m' (labToZ lr) (labToZ lrpc) 
-  (* Nothing else changed *)
-  /\ update_cache_spec_rvec cblock m m'.
+Definition handler_final_mem_matches (lrpc lr: T) (m m': memory): Z -> Z -> Prop :=
+  fun zpc zr =>
+    exists m_ext,
+      extends m m_ext /\
+      labToZ lrpc zpc m' /\
+      labToZ lr zr m' /\
+      cache_hit_read_mem cblock m' zr zpc /\
+      update_cache_spec_rvec cblock m_ext m'. (* Nothing else changed since the extension *)
 
+(* DELETE?
 Lemma genStoreResults_spec_Some': forall lr lpc,
   valid_address cblock addrTagRes m0 ->
   valid_address cblock addrTagResPC m0 ->
@@ -792,7 +1066,7 @@ Proof.
   destruct HvalidRes as [m' Hm'].
   destruct HvalidResPC as [m'' Hm''].
   destruct (load_some_store_some Hm' (Vint (labToZ lr), handlerTag)) as [m''' T'].
-  assert (TT:exists m'''', 
+  assert (TT:exists m'''',
             store cblock addrTagResPC (Vint (labToZ lpc), handlerTag) m''' = Some m'''').
     eapply load_some_store_some.
     erewrite load_store_old; eauto.
@@ -830,6 +1104,7 @@ Proof.
     exploit (load_store_old T4 cblock ofs); try congruence.
     exploit (load_store_old T' cblock ofs); try congruence.
 Qed.
+*)
 
 Lemma genError_specEscape: forall raddr (P: memory -> stack -> Prop),
   HTEscape cblock raddr genError
@@ -851,6 +1126,7 @@ Qed.
 
 Definition genFaultHandlerReturn: code := ifNZ [Ret] genError.
 
+(* ???
 Lemma genFaultHandlerReturn_specEscape_Some: forall raddr lr lpc,
   forall s0,
   HTEscape cblock raddr genFaultHandlerReturn
@@ -871,7 +1147,44 @@ Proof.
     intuition.
     jauto_set_goal; eauto.
 Qed.
+*)
 
+Lemma genFaultHandlerReturn_specEscape_Some: forall raddr (Q: memory -> stack -> Prop),
+  HTEscape cblock raddr genFaultHandlerReturn
+           (fun m s =>
+              exists s0,
+              s = (Vint 1, handlerTag) ::: CRet raddr false false :: s0 /\
+              Q m s0)
+           (fun m s  => (Q m s, Success)).
+Proof.
+  intros.
+  unfold genFaultHandlerReturn.
+  eapply HTEscape_strengthen_premise.
+  - eapply ifNZ_specEscape with (v:=1) (Pf:=fun m s => True); intros; try assumption.
+    eapply ret_specEscape; try assumption.
+    false.
+  - subst.
+    intuition. split_vc.
+Qed.
+
+Lemma genFaultHandlerReturn_specEscape_None: forall raddr s0 m0,
+ HTEscape cblock raddr genFaultHandlerReturn
+   (fun m s => (extends m0 m /\ s = (Vint 0, handlerTag) ::: s0))
+   (fun m s => (extends m0 m /\ s = s0, Failure)).
+Proof.
+  intros.
+  unfold genFaultHandlerReturn.
+  eapply HTEscape_strengthen_premise.
+  - eapply ifNZ_specEscape with (v := 0) (Pt := fun m s => True); intros; try assumption.
+    + intuition.
+    + eapply genError_specEscape.
+  - intros.
+    subst.
+    intuition.
+    jauto_set_goal; eauto.
+Qed.
+
+(* DELETE?
 Lemma genFaultHandlerReturn_specEscape_None: forall raddr s0,
  HTEscape cblock raddr genFaultHandlerReturn
    (fun (m : memory) (s : stack) => m = m0 /\ s = (Vint 0, handlerTag) ::: s0)
@@ -880,15 +1193,123 @@ Proof.
   intros.
   unfold genFaultHandlerReturn.
   eapply HTEscape_strengthen_premise.
-  - eapply ifNZ_specEscape with (v := 0) (Pt := fun m s => True); auto; intros. 
+  - eapply ifNZ_specEscape with (v := 0) (Pt := fun m s => True); auto; intros.
     + intuition.
-    + eapply genError_specEscape. 
-  - intros. 
-    subst. 
+    + eapply genError_specEscape.
+  - intros.
+    subst.
     intuition.
     jauto_set_goal; eauto.
 Qed.
- 
+*)
+
+(* MOVE *)
+Lemma extends_valid_address: forall m m' a,
+                               valid_address cblock a m ->
+                               extends m m' ->
+                               valid_address cblock a m'.
+Proof.
+  intros m m' a VALID EXT.
+  inv VALID.
+  econstructor. apply EXT. eauto.
+Qed.
+
+Lemma faultHandler_specEscape_Some: forall syscode raddr lr lpc m0,
+  INIT_MEM m0 ->
+  valid_address cblock addrTagRes m0 ->
+  valid_address cblock addrTagResPC m0 ->
+  ar = Some (lpc, lr) ->
+  forall s0,
+    HTEscape cblock raddr ((faultHandler fetch_rule_impl)++syscode)
+             (fun m s => m = m0 /\
+                         s = (CRet raddr false false::s0))
+             (fun m s => ( exists zr zpc,
+                             s = s0 /\
+                             handler_final_mem_matches lpc lr m0 m zpc zr
+                         , Success )).
+Proof.
+  intros.
+  eapply HTEscape_append.
+  unfold faultHandler.
+
+  eapply HTEscape_compose_flip.
+  eapply HTEscape_compose_flip.
+
+  eapply genFaultHandlerReturn_specEscape_Some ; eauto.
+  eapply genStoreResults_spec_Some; eauto.
+  eapply HT_consequence.
+  eapply genComputeResults_spec with
+    (I := fun m s => True)
+    (m0 := m0)
+    (s0 := CRet raddr false false :: s0)
+  ; eauto.
+  unfold extension_comp; eauto.
+  intros. intuition. substs. unfold extends; eauto.
+  simpl. intros. intuition.
+  destruct H5 as [zr [zpc Hint]]. intuition.
+  exists (CRet raddr false false :: s0).
+  exists zr ; exists zpc.
+  intuition; eauto using extends_valid_address.
+
+  assert (Hm'm'':
+            exists m' m'',
+              store cblock addrTagRes (Vint zr, t1) m = Some m' /\
+              store cblock addrTagResPC (Vint zpc, t2) m' = Some m'').
+  {
+   exploit (extends_valid_address m0 m addrTagRes); eauto. intros HvalidRes.
+   exploit (extends_valid_address m0 m addrTagResPC); eauto. intros HvalidResPC.
+   eapply (valid_store cblock addrTagRes (Vint zr,t1)) in HvalidRes.
+   destruct HvalidRes as [m' ?].
+   eapply valid_address_upd with (a:= addrTagResPC) in HvalidResPC; eauto.
+   eapply valid_store in HvalidResPC.
+   destruct HvalidResPC as [m'' ?]; eauto.
+  }
+
+  destruct Hm'm'' as [m' [m'' [Hm' Hm'']]].
+  assert (Hup: mem_eq_except_cache cblock m m''); eauto.
+  {
+    econstructor.
+    - eapply INIT_MEM_def_on_cache; eauto using extension_comp_INIT_MEM.
+    - intros.
+      cut (load b addr m'' = load b addr m); try congruence.
+      transitivity (load b addr m'); eapply load_store_old; eauto; congruence.
+  }
+  do 2 eexists ; intuition; eauto.
+  {  unfold labToZ_rule_res in *.
+     rewrite H2 in *. intuition; eapply labToZ_cache; eauto.
+  }
+  eexists; intuition; eauto.
+  exists zr ; exists zpc ; intuition; eauto.
+  exists m. intuition; eauto.
+  {  unfold labToZ_rule_res in *.
+     rewrite H2 in *. intuition; eapply labToZ_cache; eauto.
+  }
+  {  unfold labToZ_rule_res in *.
+     rewrite H2 in *. intuition; eapply labToZ_cache; eauto.
+  }
+  { assert (Hm''' : load cblock addrTagRes m'' = Some (Vint zr, t1)).
+    { eapply load_store_new in Hm'.
+      erewrite load_store_old; eauto.
+      compute; congruence. }
+    clear Hm'.
+    eapply load_store_new in Hm''.
+    unfold load, cache_hit_read_mem in *.
+    destruct (Mem.get_frame m'' cblock) as [fr|]; try congruence.
+    econstructor; econstructor; eauto.
+  }
+  (* AAA: Probably need to change definition of update_cache_spec_rvec and mem_eq_except_cache *)
+  unfold update_cache_spec_rvec.
+  split.
+
+
+  intros; jauto_set_hyps; intros.
+  eapply transitivity.
+  eapply update_list_Z_spec2; eauto.
+  eapply update_list_Z_spec2; eauto.
+Qed.
+
+(* AAA: Stopped transcription here *)
+
 Lemma faultHandler_specEscape_Some: forall raddr lr lpc,
   valid_address cblock addrTagRes m0 ->
   valid_address cblock addrTagResPC m0 ->
@@ -911,7 +1332,7 @@ Proof.
 Qed.
 
 Lemma faultHandler_specEscape_None: forall raddr,
-  ar = None -> 
+  ar = None ->
   forall s0,
     HTEscape cblock raddr (faultHandler fetch_rule_impl)
              (fun m s => m = m0 /\ s = s0)
@@ -951,28 +1372,28 @@ Proof.
   destruct (Mem.get_frame m cblock) eqn:E; try (intuition; fail).
 
   assert (valid_address cblock addrTagRes m).
-    inv INPUT. inv TAGR. 
+    inv INPUT. inv TAGR.
     econstructor.
     unfold load; rewrite E.
-    edestruct index_list_Z_valid; eauto. 
+    edestruct index_list_Z_valid; eauto.
   assert (valid_address cblock addrTagResPC m).
-    inv INPUT. inv TAGRPC. 
+    inv INPUT. inv TAGRPC.
     econstructor.
     unfold load; rewrite E.
-    edestruct index_list_Z_valid; eauto. 
+    edestruct index_list_Z_valid; eauto.
 
-  edestruct (faultHandler_specEscape_Some get_rule opcode vls pcl m) 
-      as [stk1 [cache1 [pc1 [priv1 [[P1 P2] [P3 P4]]]]]]; eauto. 
-   eapply init_enough; auto. 
+  edestruct (faultHandler_specEscape_Some get_rule opcode vls pcl m)
+      as [stk1 [cache1 [pc1 [priv1 [[P1 P2] [P3 P4]]]]]]; eauto.
+   eapply init_enough; auto.
   unfold Concrete.cache_hit_mem; rewrite E; auto.
-  apply code_at_id. 
-  exists cache1. 
-  inversion P3.  subst. 
+  apply code_at_id.
+  exists cache1.
+  inversion P3.  subst.
   intuition.
-  apply P4. 
-Qed.  
-              
-Theorem handler_correct_fail : 
+  apply P4.
+Qed.
+
+Theorem handler_correct_fail :
   forall opcode vls pcl m raddr s i,
   forall (INPUT: cache_hit_mem m (opCodeToZ opcode) (labsToZs vls) (labToZ pcl))
          (RULE: apply_rule (projT2 (get_rule opcode)) pcl vls = None),
@@ -981,17 +1402,15 @@ Theorem handler_correct_fail :
                  (CState m handler i (CRet raddr false false::s) (0,handlerTag) true)
                  (CState m handler i st (-1,handlerTag) true).
 Proof.
-  intros.   
+  intros.
   edestruct (faultHandler_specEscape_None get_rule opcode vls pcl m) with (raddr := (0,0))
-      as [stk1 [cache1 [pc1 [priv1 [[P1 P2] [P3 P4]]]]]]; eauto. 
-   eapply init_enough; eauto. 
-   eapply code_at_id. 
-  inv P3. 
+      as [stk1 [cache1 [pc1 [priv1 [[P1 P2] [P3 P4]]]]]]; eauto.
+   eapply init_enough; eauto.
+   eapply code_at_id.
+  inv P3.
   eexists; eauto.
 Qed.
 
 End HandlerCorrect.
 
 End TMU.
-
-
